iris/ProofSysWait.v
@@ -301,7 +301,9 @@ Section ProofSysWait.
               Hj Hgl (sw_Kkw av Hav) Heb
               with "Hcg Hcpu Htext Hpc Hprocs Hlk Henv Hpriv").
     all: try lkbelow.
-    iIntros (CID11 Hk11 Mkw P' rv d bs) "%Hkw %Hext %Hdle Hcg Hcpu Hpc Hpriv".
+    iIntros (CID11 Hk11 Mkw P' rv d bs)
+      "%Hkw %Hext %Hdle %Hnull Hcg Hcpu Hpc Hpriv".
+    rewrite HB2a0 in Hnull.
     destruct Hkw as (HcsKw & HKwa0).
     iEval (rewrite HB2a0) in "Hpriv".
     assert (Hpp1a : ret_pc (B2 !!! Regidx Rra) = mword_of_int (SW + 0x1a))
@@ -420,7 +422,8 @@ Section ProofSysWait.
       rewrite /M1 upd_ne; [| congruence]. reflexivity. }
     iDestruct (cpu_own_transport CID11 CID15 0%nat eb pj b ltac:(wp_next_chain) with "Hcpu") as "Hcpu".
     iSpecialize ("Hcont" $! CID15 with "[%]"); [wp_next_chain|].
-    iApply ("Hcont" $! E2 P' rv d bs with "[%] [%] [%] Hcg Hcpu Hpc Hpriv").
+    iApply ("Hcont" $! E2 P' rv d bs
+              with "[%] [%] [%] [%] Hcg Hcpu Hpc Hpriv").
     { split; [| exact HE2a0].
       unfold callee_saved.
       split; [exact HE2sp|]. split; [exact HE2s0|].
@@ -428,6 +431,7 @@ Section ProofSysWait.
       apply Hthr; vm_compute; first [reflexivity | discriminate]. }
     { exact Hext. }
     { exact Hdle. }
+    { exact Hnull. }
   Qed.
 
 End ProofSysWait.
